src/basic/FStarC.Errors.Codes.fst
@@ -403,4 +403,5 @@ let default_settings : list error_setting =
     Error_CustardEntryNotFound                         , CAlwaysError, 385;
     Error_CustardBadFloatWidth                         , CAlwaysError, 386;
     Warning_CustardFloatVocabulary                     , CWarning, 387;
+    Error_CustardPolyExternalUnused                    , CAlwaysError, 388;
     ]
